Timepiece.v
@@ -15,9 +15,11 @@ Section timepiece.
   Variable F : Edge -> S -> S.
 
   Definition φ := S -> Prop.
-  Definition A := nat -> φ.
+  Definition Q := nat -> φ.
 
-  Definition true_inv : A := fun t s => True.
+  Definition true_inv : Q := fun t s => True.
+
+  Variable A : Node -> Q.
 
   (* Computing a new route at a node given routes of its neighbors. *)
   Definition updated_state (node : Node)
@@ -32,7 +34,7 @@ Section timepiece.
       | Datatypes.S t' => updated_state node (map (fun m => (m, σ g m t')) (nth node g nil))
     end.
 
-  Definition initial_condition (node : Node) (invariant : A) := invariant 0 (I node).
+  Definition initial_condition (node : Node) := A node 0 (I node).
 
   (* A helper definition for writing out the inductive condition with times
      erased: all invariants are specified as [S -> Prop] functions. *)
@@ -46,36 +48,40 @@ Section timepiece.
     (node_invariant (updated_state node neighbors)).
 
   (* The original inductive condition for a node [n]. *)
-  Definition inductive_condition (n : Node) (node_invariant : A)
-                                 (neighbors : list Node) (neighbor_invariants : list A) :=
+  Definition inductive_condition
+    (n : Node) (neighbors : list Node) :=
     forall (t : nat) (states : list S),
       length states = length neighbors ->
       inductive_condition_untimed
-        n (node_invariant (1 + t))
-        (combine neighbors states) (map (fun a => (a t)) neighbor_invariants).
+        n (A n (1 + t))
+        (combine neighbors states) (map (fun m => (A m t)) neighbors).
 
   Definition inductive_invariant
-    (n : Node) (node_invariant : A) (neighbors : list Node) (neighbor_invariants : list A) :=
-    initial_condition n node_invariant /\ inductive_condition n node_invariant neighbors neighbor_invariants.
+    (n : Node) (neighbors : list Node) :=
+    initial_condition n /\ inductive_condition n neighbors.
 
   Lemma inductive_condition_is_sound :
-    forall (g : Graph) (invariants : list A),
-      length g = length invariants ->
-      forall (v : Node),
+    forall (g : Graph) (v : Node),
         v < length g ->
-        inductive_invariant
-          v (nth v invariants true_inv) (nth v g nil)
-          (map (fun nbr => (nth nbr invariants true_inv)) (nth v g nil)) ->
-        forall (t : nat), (nth v invariants true_inv) t (σ g v t).
+        Forall (fun u => u < length g) (nth v g nil) ->
+        inductive_invariant v (nth v g nil) ->
+        forall (t : nat), A v t (σ g v t).
   Proof.
-    intros g invariants Hglen v Hving Hindinv t.
+    intros g v Hving Huing Hindinv t.
     generalize dependent v.
-    induction t; intros v Hving [Hinitial Hinductive].
+    induction t; intros v Hving Huing [Hinitial Hinductive].
     - assumption. (* by Hinitial *)
     - simpl.
-      remember (nth v invariants true_inv) as a.
+      induction (nth v g nil).
+      + simpl. unfold inductive_condition in Hinductive.
+        simpl in Hinductive. unfold inductive_condition_untimed in Hinductive.
+        apply (Hinductive t nil); auto.
+        apply Forall_nil.
+      + simpl in *. unfold inductive_condition in Hinductive.
+        unfold inductive_condition_untimed in Hinductive.
+        simpl in Hinductive.
+        admit.
       (* now need to connect the state with the invariant *)
-      admit.
   Admitted.
 
 End timepiece.
